src/ocaml_host.ml
@@ -1,0 +1,41 @@
+open Utils
+
+let clock_ms () = 
+  let time = Unix.gettimeofday() in
+      int_of_float (time *. 1000.0)
+
+module Ocaml_host: Extract.Parametric_host = struct
+
+  type host_function = int
+  let host_function_eq_dec a b = (a = b)
+
+  let hfc = host_function_eq_dec
+
+  type host_state_type = unit
+
+  let host_apply_pure hs s ft hf vs = 
+    match Obj.magic hf with
+    | 0 -> 
+      let ms = clock_ms () in
+        ((), Some (s, Extract.Result_values [Extract.Utility.vali64_of_Z (z_of_int ms)]))
+    | _ -> 
+      assert false
+
+end
+
+let starting_wasm_host_store = 
+  let hf0 = Extract.FC_func_host (Extract.Tf ([], [Extract.T_num Extract.T_i64]), Obj.magic 0) in
+  let starting_wasm_store = 
+    {Extract.s_funcs = [hf0]; 
+     Extract.s_tables = []; 
+     Extract.s_mems = []; 
+     Extract.s_globals = []; 
+     Extract.s_elems = []; 
+     Extract.s_datas = []
+    } 
+  in
+  let env_module_exps = StringMap.add "clock_ms"  (Extract.EV_func (z_of_int 0)) Utils.StringMap.empty in 
+  let module_extern_store = StringMap.add "env" env_module_exps Utils.StringMap.empty in
+  let module_name_store = StringMap.add "env" "env" Utils.StringMap.empty in
+  let starting_host_store = (module_extern_store, module_name_store) in
+  (starting_wasm_store, starting_host_store)
