src/utils.ml
@@ -7,3 +7,5 @@ let int_of_z z =
   if Big_int_Z.is_int_big_int z then 
     Big_int_Z.int_of_big_int z
 else invalid_arg "int_of_z overflow"
+
+module StringMap = Map.Make(String);;
