src/utils.mli
@@ -6,3 +6,6 @@ val string_of_char : char -> string
 val z_of_int: int -> Big_int_Z.big_int
 
 val int_of_z: Big_int_Z.big_int -> int
+
+(* Type of the host extern val store *)
+module StringMap : Map.S with type key = string
