src/wasm_coq_interpreter.ml
@@ -19,9 +19,8 @@ let process_args_and_run verbosity text no_exec max_call_depth srcs func_name sr
           s) srcs in
     let mnames = List.map extract_module_name srcs in
     let* modules = parse_modules verbosity text files in
-    let starting_host_store = (Execute.StringMap.empty, Execute.StringMap.empty) in
-    let starting_store = empty_store_record in
-    let* (exts, s) = Execute.instantiate_modules verbosity starting_host_store starting_store mnames modules in
+    let (starting_wasm_store, starting_host_store) = Ocaml_host.starting_wasm_host_store in
+    let* (exts, s) = Execute.instantiate_modules verbosity starting_host_store starting_wasm_store mnames modules in
     let* args = parse_args arg_strings in
     (** Running. *)
     if no_exec then
