theories/extraction_instance.v
@@ -1,8 +1,8 @@
 (* The setup for extraction *)
-From Coq Require Import String.
+From Coq Require Import String ZArith.
 From mathcomp Require Import ssreflect ssrfun ssrnat ssrbool eqtype seq.
 From HB Require Import structures.
-From Wasm Require Import memory host interpreter_ctx instantiation_func pp.
+From Wasm Require Import numerics memory host interpreter_ctx instantiation_func pp.
 From ExtLib Require Import Structures.Monad.
 From ExtLib Require Import IdentityMonad.
 
@@ -14,8 +14,8 @@ Module Memory_instance.
   
 End Memory_instance.
 
-Module Extraction_instance.
-
+(*
+(* Host instance with no host functions. *)
 Section DummyHost.
 
 Existing Instance Memory_instance.memory_instance.
@@ -60,19 +60,94 @@ Proof.
 Defined.
 
 End DummyHost.
+ *)
+  
+  (* A more general extraction that allows non-trivial host functions, extracting the interpreter as a functor-like module. Not using the monadic design yet as that requires corresponding changes to the interpreter as well. *)
+  Module Type Parametric_host.
 
+    Parameter host_function: Type.
+
+    Parameter host_function_eq_dec: forall (a b: host_function),
+        {a = b} + {a <> b}.
+
+    #[export]
+      Instance hfc: host_function_class := Build_host_function_class host_function_eq_dec.
+
+    Parameter host_state_type : Type.
+
+    (* Host function application are left as parameters and must be realised in a separate file in extraction. *)
+    (* Migrate to monadic host operations when the interpreter updates to itree *)
+    Parameter host_apply_pure: host_state_type -> store_record -> function_type -> host_function -> seq value -> (host_state_type * option (store_record * result)).
+
+    (* However, such a parametric host cannot be proven to respect Wasm's store invariant, as they will be formulated in OCaml. *)
+    Axiom host_application_extension : forall hs s ft h vs hs' s' r,
+        host_apply_pure hs s ft h vs = (hs', Some (s', r)) ->
+        store_extension s s'.
+
+    Axiom host_application_typing : forall hs s ft h vs hs' s' r,
+        host_apply_pure hs s ft h vs = (hs', Some (s', r)) ->
+        store_typing s ->
+        store_typing s'.
+
+    Axiom host_application_respect : forall hs s ts1 ts2 h vs hs' s' r,
+        host_apply_pure hs s (Tf ts1 ts2) h vs = (hs', Some (s', r)) ->
+        result_types_agree s' ts2 r.
+
+  End Parametric_host.
+
+  Module Monadic_host (PH: Parametric_host).
+
+    Include PH.
+    
+    Definition host_event := ident.
+    Definition host_ret := @ret _ Monad_ident.
+    Definition host_bind := @bind _ Monad_ident.
+
+  End Monadic_host.
+Module Utility.
+  
+  Definition vali32_of_Z (z: Z) : value :=
+    VAL_num (VAL_int32 (Wasm_int.int_of_Z i32m z)).
+  
+  Definition vali64_of_Z (z: Z) : value :=
+    VAL_num (VAL_int64 (Wasm_int.int_of_Z i64m z)).
+  
+End Utility.
+
+
+Module Extraction_instance (PH: Parametric_host).
+
+Export PH.
+
+#[export]
+Instance host_instance : host.
+Proof.
+  refine {|
+      host_state := host_state_type;
+      host_application hs s ft hf vs hs' res := host_apply_pure hs s ft hf vs = (hs', res)
+    |}.
+  - intros; by eapply host_application_extension; eauto.
+  - intros; by eapply host_application_typing; eauto.
+  - intros; by eapply host_application_respect; eauto.
+Defined.
+
+Definition host_application_impl_correct :
+  (forall hs s ft hf vs hs' hres, (host_apply_pure hs s ft hf vs = (hs', hres)) -> host_application hs s ft hf vs hs' hres).
+Proof.
+  done.
+Defined.
 
 Section Interpreter_ctx_extract.
 
-  Definition empty_frame := empty_frame.
-
-  Definition store_record := store_record.
+Definition empty_frame := empty_frame.
+  
+Definition store_record := store_record.
   
 Definition cfg_tuple_ctx : Type := cfg_tuple_ctx.
 
 Definition run_step_ctx_result : host_state -> cfg_tuple_ctx -> BinNums.N -> Type := run_step_ctx_result.
 
-Definition run_one_step (cfg: cfg_tuple_ctx) (d: BinNums.N) : run_step_ctx_result tt cfg d := run_one_step host_application_impl_correct tt cfg d.
+Definition run_one_step (hs: host_state) (cfg: cfg_tuple_ctx) (d: BinNums.N) : run_step_ctx_result hs cfg d := run_one_step host_application_impl_correct hs cfg d.
 
 Definition run_v_init : store_record -> list administrative_instruction -> option cfg_tuple_ctx := run_v_init.
 
@@ -89,7 +164,7 @@ Definition pp_store := pp_store.
 
 Definition pp_cfg_tuple_ctx_except_store := pp_cfg_tuple_ctx_except_store.
 
-Definition pp_res_cfg_except_store {cfg: cfg_tuple_ctx} {d: BinNums.N} (res: run_step_ctx_result tt cfg d) := pp_res_cfg_except_store res.
+Definition pp_res_cfg_except_store {hs: host_state} {cfg: cfg_tuple_ctx} {d: BinNums.N} (res: run_step_ctx_result hs cfg d) := pp_res_cfg_except_store res.
 
 Definition pp_administrative_instructions := pp_administrative_instructions.
 
@@ -110,8 +185,8 @@ Definition empty_store_record : store_record := {|
   |}.
 
 (* Provide a unit host state and convert the starting expression to administrative *)
-Definition interp_instantiate_wrapper (s: store_record) (m : module) (v_imps: list extern_value) : option config_tuple * string :=
-  match interp_instantiate tt s m v_imps with
+Definition interp_instantiate_wrapper (hs: host_state) (s: store_record) (m : module) (v_imps: list extern_value) : option config_tuple * string :=
+  match interp_instantiate hs s m v_imps with
   | (Some (hs', s', f, bes), str) => (Some (s', (f, to_e_list bes)), str)
   | (None, str) => (None, str)
   end.
@@ -150,6 +225,16 @@ Definition wasm_global_get (s: store_record) (ext: extern_value) : option value 
   end.
 
 End Instantiation_func_extract.
+
+Section Utility.
+
+  Definition vali32_of_Z (z: Z) : value :=
+    VAL_num (VAL_int32 (Wasm_int.int_of_Z i32m z)).
+  
+  Definition vali64_of_Z (z: Z) : value :=
+    VAL_num (VAL_int64 (Wasm_int.int_of_Z i64m z)).
+  
+End Utility.
 
 Section Wast.
   
